\section{Geometry}

\subsection{Pythagoras' Theorem} \label{sec_pythagoras}

%FIXME add diagram

If a triangle has sides \(a\), \(b\), \(c\) opposed by angles \(A\), \(B\),
\(C\), then
\begin{equation*}
 C = \frac 12 \pi \iff a^2 + b^2 = c^2
\end{equation*}

\subsection{Angles in a Polygon} \label{sec_geom_polygon_angles}

\subsection{Area of a Circle}

%FIXME add diagram

\begin{theorem}[Area of a circle]
 The area of a circle of radius \(r\) is given by
 \begin{equation*}
  A = \pi r^2
 \end{equation*}
\end{theorem}
\begin{proof}
 From the definition of a circle as the set of points equidistant from a
 centre point, we form the equation of a circle using \ref{sec_pythagoras}:
 \(x^2 + y^2 = r^2\), where the centre is \((0, 0)\) and the radius is \(r\).

 We can find half the area enclosed by the curve by integrating:
 \begin{equation*}
  \frac 12 A = \integ[-r]<r>{\sqrt{r^2 - x^2}}{x}
 \end{equation*}
 We use the substitution (\ref{sec_calc_trig_substitution})
 \(x = r \cos \theta \implies \dv<x>{\theta} = -r \sin \theta\) so that
 \begin{equation*}
  \frac 12 A = \integ[\arccos -1]<\arccos 1>
  {r\sqrt{1 - \cos^2 \theta} \cdot -r \sin \theta}{\theta}
  = -\integ[\pi]<0>{r^2 \sin^2 \theta}{\theta}
 \end{equation*}
 by \ref{sec_trig_pythag}. We use \ref{sec_trig_double_angle} to derive
 \begin{align*}
  \frac 12 A &= -\integ[\pi]<0>
  {r^2 \frac 12 (1 - \cos 2 \theta)}{\theta} \implies
  A = r^2 \integ[0]<\pi>{(1 - \cos 2 \theta)}{\theta} =
  r^2\parens[\Big]{\theta - \frac 12 \sin 2 \theta}\eval_0^\pi \\
  &= r^2 \parens[\Big]{\pi - \frac 12 \sin 2 \pi -
  \parens[\Big]{0 - \frac 12 \sin 0}} = \pi r^2 \qedhere
 \end{align*}
\end{proof}
\begin{proof}[Alternative proof]
 One might alternatively use the parametric form of a circle,
 \(y = r \sin \theta\) and \(x = r \cos \theta\)
 (note that \(x^2 + y^2 = r^2(\sin^2 \theta + \cos^2 \theta) = r^2\)
 (\ref{sec_trig_pythag})), and calculate the area using
 \ref{sec_calc_parametric_area}:
 \begin{align*}
  A &= \integ[0]<2\pi>
  {r \sin \theta \cdot -r \sin \theta}{\theta} =
  \frac 12 r^2 \integ[0]<2\pi>{(1 - \cos 2 \theta)}{\theta} =
  \frac 12 r^2 \parens[\Big]{\theta - \frac 12 \sin 2 \theta}\eval_0^{2\pi} \\
  &= \frac 12 r^2 \parens[\Big]{2\pi - \frac 12 \sin 4 \pi -
  (0 - \sin 0)} = \pi r^2 \qedhere
 \end{align*}
\end{proof}

\subsection{Volume of a sphere}

\subsection{Circle Theorems}
